AwsCryptographicMaterialProviders/dafny/AwsCryptographyKeyStore/src/GetKeys.dfy
@@ -2,432 +2,169 @@
 // SPDX-License-Identifier: Apache-2.0
 
 include "../Model/AwsCryptographyKeyStoreTypes.dfy"
-include "CreateKeyStoreTable.dfy"
-
-include "../../AwsCryptographicMaterialProviders/src/AwsArnParsing.dfy"
-include "../../AwsCryptographicMaterialProviders/src/Keyrings/AwsKms/AwsKmsUtils.dfy"
+include "Structure.dfy"
+include "DDBKeystoreOperations.dfy"
+include "KMSKeystoreOperations.dfy"
 
 module GetKeys {
   import opened StandardLibrary
   import opened Wrappers
-  import opened AwsArnParsing
-  import opened AwsKmsUtils
-  import opened CreateKeyStoreTable
   import opened Seq
+
+  import Structure
+  import KMSKeystoreOperations
+  import DDBKeystoreOperations
+
   import Types = AwsCryptographyKeyStoreTypes
   import DDB = ComAmazonawsDynamodbTypes
   import KMS = ComAmazonawsKmsTypes
-  import MPL = AwsCryptographyMaterialProvidersTypes
-
-  const TYPE_FIELD := "type";
-  const BRANCH_KEY_TYPE_PREFIX := "version:";
-  const BRANCH_KEY_IDENTIFIER_FIELD := "branch-key-id";
-  const TABLE_FIELD := "tablename";
-  const KMS_FIELD := "kms-arn";
-
-  const BRANCH_KEY_FIELD := "enc";
-
-  const STATUS_BRANCH_KEY_ID_MATCH_EXPRESSION := "#branch_key_id = :branch_key_id and #status = :status";
-  const EXPRESSION_ATTRIBUTE_NAMES := map[
-                                        "#branch_key_id" := "branch-key-id",
-                                        "#status"       := "status"
-                                      ];
-  const EXPRESSION_ATTRIBUTE_VALUE_STATUS_KEY := ":status";
-  const STATUS_ACTIVE := "ACTIVE";
-  const EXPRESSION_ATTRIBUTE_VALUE_BRANCH_KEY := ":branch_key_id";
-
-  type baseKeyStoreItem = m: DDB.AttributeMap | baseKeyStoreItemHasRequiredAttributes?(m) witness *
-  predicate method baseKeyStoreItemHasRequiredAttributes?(m: DDB.AttributeMap) {
-    && "branch-key-id" in m && m["branch-key-id"].S?
-    && "type" in m && m["type"].S?
-    && "status" in m && m["status"].S?
-    && "create-time" in m && m["create-time"].S?
-    && "hierarchy-version" in m && m["hierarchy-version"].N?
-    && KMS_FIELD in m && m[KMS_FIELD].S?
-    && BRANCH_KEY_FIELD in m && m[BRANCH_KEY_FIELD].B?
-    && KMS.IsValid_CiphertextType(m[BRANCH_KEY_FIELD].B)
-    && var tmpM := m - {BRANCH_KEY_FIELD};
-    && forall k | k in tmpM :: ValueToString(tmpM[k]).Success?
-  }
-  predicate method validBeaconKeyItem?(m: DDB.AttributeMap) {
-    && baseKeyStoreItemHasRequiredAttributes?(m)
-    && m["type"].S == "beacon:true"
-    && m["status"].S == "SEARCH"
-  }
-
-  type branchKeyItem = m: DDB.AttributeMap | validActiveBranchKey?(m) witness *
-  predicate method validActiveBranchKey?(m: DDB.AttributeMap) {
-    && baseKeyStoreItemHasRequiredAttributes?(m)
-    && m["status"].S == "ACTIVE"
-    && |m["type"].S| > |BRANCH_KEY_TYPE_PREFIX|
-  }
-
-  type versionBranchKeyItem = m: DDB.AttributeMap | validVersionBranchKey?(m) witness *
-  predicate method validVersionBranchKey?(m: DDB.AttributeMap) {
-    && baseKeyStoreItemHasRequiredAttributes?(m)
-    && (m["status"].S == "ACTIVE" || m["status"].S == "DECRYPT_ONLY")
-    && |m["type"].S| > |BRANCH_KEY_TYPE_PREFIX|
-  }
-
-  function method ValueToString(a: DDB.AttributeValue): Result<string, Types.Error>
-  {
-    match a {
-      case S(s) => Success(a.S)
-      case N(n) => Success(a.N)
-      // For now we only support AttributeValues that are either String or Number
-      // AttributeValues, we have not specified how to represent attributes other than these
-      // two, we SHOULD include them but we have to agree how to turn the underlying
-      // type into a string/bytes so that they could be turned to UTF8 bytes to pass KMS.
-      case _ => Failure(E("Type not supported"))
-    }
-  }
 
   method GetActiveKeyAndUnwrap(
     input: Types.GetActiveBranchKeyInput,
     tableName: DDB.TableName,
     logicalKeyStoreName: string,
-    kmsKeyArn: Types.KmsKeyArn,
+    kmsConfiguration: Types.KMSConfiguration,
     grantTokens: KMS.GrantTokenList,
     kmsClient: KMS.IKMSClient,
     ddbClient: DDB.IDynamoDBClient
   )
-    returns (res: Result<Types.GetActiveBranchKeyOutput, Types.Error>)
+    returns (output: Result<Types.GetActiveBranchKeyOutput, Types.Error>)
     requires kmsClient.ValidState() && ddbClient.ValidState()
-    requires DDB.IsValid_TableName(tableName)
-    requires KMS.IsValid_KeyIdType(kmsKeyArn)
     modifies ddbClient.Modifies, kmsClient.Modifies
     ensures ddbClient.ValidState() && kmsClient.ValidState()
-  {
-    var maybeQueryResponse := QueryForActiveBranchKey(input.branchKeyIdentifier, tableName, ddbClient);
-    var queryResponse :- maybeQueryResponse
-    .MapFailure(e => Types.ComAmazonawsDynamodb(ComAmazonawsDynamodb := e));
 
-    :- Need(
-      && queryResponse.Items.Some?
-      && |queryResponse.Items.value| > 0,
-      E("No item found for corresponding branch key identifier.")
-    );
+    ensures output.Success? ==>
+              input.branchKeyIdentifier == output.value.branchKeyMaterials.branchKeyIdentifier
 
-    :- Need(
-      forall resp <- queryResponse.Items.value :: validActiveBranchKey?(resp),
-      E("Malformed Branch Key entry")
-    );
+    {
 
-    var branchKeyRecord := SortByTime(queryResponse.Items.value);
+      var branchKeyItem :- DDBKeystoreOperations.GetActiveBranchKeyItem(
+        input.branchKeyIdentifier,
+        tableName,
+        ddbClient
+      );
 
-    var branchKeyResponse :- decryptKeyStoreItem(branchKeyRecord, kmsKeyArn, grantTokens, logicalKeyStoreName, kmsClient);
-    var branchKeyVersion := branchKeyRecord["type"].S[|BRANCH_KEY_TYPE_PREFIX|..];
-    var branchKeyVersionUtf8 :- UTF8.Encode(branchKeyVersion).MapFailure(e => E(e));
+      var encryptionContext := Structure.ToBranchKeyContext(branchKeyItem, logicalKeyStoreName);
 
-    return Success(Types.GetActiveBranchKeyOutput(
-                     branchKeyMaterials := Types.BranchKeyMaterials(
-                       branchKeyIdentifier := input.branchKeyIdentifier,
-                       branchKeyVersion := branchKeyVersionUtf8,
-                       branchKey := branchKeyResponse.Plaintext.value
-                     )
-                   ));
-  }
+      :- Need(
+        KMSKeystoreOperations.AttemptKmsOperation?(kmsConfiguration, encryptionContext),
+        Types.KeyStoreException( message := "AWS KMS Key ARN does not match configured value")
+      );
 
-  method QueryForActiveBranchKey(branchKeyId: string, ddbTableName: DDB.TableName, ddbClient: DDB.IDynamoDBClient)
-    returns (res: Result<DDB.QueryOutput, DDB.Error>)
-    requires ddbClient.ValidState()
-    modifies ddbClient.Modifies
-    ensures ddbClient.ValidState()
-    ensures
-      && |ddbClient.History.Query| > 0
-      && var ddbOperationOutput := Last(ddbClient.History.Query).output;
-      && ddbOperationOutput.Failure?
-      ==> res.Failure?
-    ensures res.Success? ==>
-              && |ddbClient.History.Query| > 0
-              && var ddbOperationInput := Last(ddbClient.History.Query).input;
-              && var ddbOperationOutput := Last(ddbClient.History.Query).output;
-              && var expressionAttributeValues: DDB.AttributeMap := map[
-                                                                      EXPRESSION_ATTRIBUTE_VALUE_BRANCH_KEY := DDB.AttributeValue.S(branchKeyId),
-                                                                      EXPRESSION_ATTRIBUTE_VALUE_STATUS_KEY := DDB.AttributeValue.S(STATUS_ACTIVE)];
-              && ddbOperationOutput.Success?
-              && ddbOperationInput.TableName == ddbTableName
-              && ddbOperationInput.IndexName.Some?
-              && ddbOperationInput.KeyConditionExpression.Some?
-              && ddbOperationInput.KeyConditionExpression.value == STATUS_BRANCH_KEY_ID_MATCH_EXPRESSION
-              && ddbOperationInput.ExpressionAttributeNames.Some?
-              && ddbOperationInput.ExpressionAttributeNames.value == EXPRESSION_ATTRIBUTE_NAMES
-              && ddbOperationInput.ExpressionAttributeValues.Some?
-              && ddbOperationInput.ExpressionAttributeValues.value == expressionAttributeValues
-              && ddbOperationOutput.value == res.value
-  {
-    var expressionAttributeValues : DDB.AttributeMap := map[
-      EXPRESSION_ATTRIBUTE_VALUE_BRANCH_KEY := DDB.AttributeValue.S(branchKeyId),
-      EXPRESSION_ATTRIBUTE_VALUE_STATUS_KEY := DDB.AttributeValue.S(STATUS_ACTIVE)
-    ];
+      var branchKey :- KMSKeystoreOperations.DecryptKey(
+        encryptionContext,
+        branchKeyItem[Structure.BRANCH_KEY_FIELD].B,
+        kmsConfiguration,
+        grantTokens,
+        kmsClient
+      );
 
-    var queryInput := DDB.QueryInput(
-      TableName := ddbTableName,
-      IndexName := None,
-      Select := None,
-      AttributesToGet := None,
-      Limit := None,
-      ConsistentRead :=  None,
-      KeyConditions := None,
-      QueryFilter := None,
-      ConditionalOperator := None,
-      ScanIndexForward := None,
-      ExclusiveStartKey := None,
-      ReturnConsumedCapacity :=  None,
-      ProjectionExpression := None,
-      FilterExpression := None,
-      KeyConditionExpression := Some(STATUS_BRANCH_KEY_ID_MATCH_EXPRESSION),
-      ExpressionAttributeNames := Some(EXPRESSION_ATTRIBUTE_NAMES),
-      ExpressionAttributeValues := Some(expressionAttributeValues)
-    );
+      var branchKeyMaterials :- Structure.ToBranchKeyMaterials(
+        encryptionContext,
+        branchKey.Plaintext.value
+      );
 
-    var queryResponse :- ddbClient.Query(queryInput);
+      return Success(Types.GetActiveBranchKeyOutput(
+                       branchKeyMaterials := branchKeyMaterials
+                     ));
 
-    res := Success(queryResponse);
-  }
+    }
 
   method GetBranchKeyVersion(
     input: Types.GetBranchKeyVersionInput,
     tableName: DDB.TableName,
     logicalKeyStoreName: string,
-    kmsKeyArn: Types.KmsKeyArn,
+    kmsConfiguration: Types.KMSConfiguration,
     grantTokens: KMS.GrantTokenList,
     kmsClient: KMS.IKMSClient,
     ddbClient: DDB.IDynamoDBClient
   )
-    returns (res: Result<Types.GetBranchKeyVersionOutput, Types.Error>)
+    returns (output: Result<Types.GetBranchKeyVersionOutput, Types.Error>)
     requires kmsClient.ValidState() && ddbClient.ValidState()
-    requires DDB.IsValid_TableName(tableName)
-    requires KMS.IsValid_KeyIdType(kmsKeyArn)
     modifies ddbClient.Modifies, kmsClient.Modifies
     ensures ddbClient.ValidState() && kmsClient.ValidState()
-  {
-    var dynamoDbKey: DDB.Key := map[
-      BRANCH_KEY_IDENTIFIER_FIELD := DDB.AttributeValue.S(input.branchKeyIdentifier),
-      TYPE_FIELD := DDB.AttributeValue.S(BRANCH_KEY_TYPE_PREFIX + input.branchKeyVersion)
-    ];
-    var ItemRequest := DDB.GetItemInput(
-      Key := dynamoDbKey,
-      TableName := tableName,
-      AttributesToGet := None,
-      ConsistentRead :=  None,
-      ReturnConsumedCapacity := None,
-      ProjectionExpression := None,
-      ExpressionAttributeNames := None
-    );
+    ensures output.Success? ==>
+              && input.branchKeyIdentifier == output.value.branchKeyMaterials.branchKeyIdentifier
+    // && TODO add version info
+    {
 
-    var maybeGetItem := ddbClient.GetItem(ItemRequest);
-    var getItemResponse :- maybeGetItem
-    .MapFailure(e => Types.ComAmazonawsDynamodb(ComAmazonawsDynamodb := e));
+      var branchKeyItem :- DDBKeystoreOperations.GetVersionBranchKeyItem(
+        input.branchKeyIdentifier,
+        input.branchKeyVersion,
+        tableName,
+        ddbClient
+      );
 
-    :- Need(
-      getItemResponse.Item.Some?,
-      E("No item found for corresponding branch key identifier.")
-    );
+      var encryptionContext := Structure.ToBranchKeyContext(branchKeyItem, logicalKeyStoreName);
 
-    :- Need(
-      validVersionBranchKey?(getItemResponse.Item.value),
-      E("Malformed Branch Key entry")
-    );
+      :- Need(
+        KMSKeystoreOperations.AttemptKmsOperation?(kmsConfiguration, encryptionContext),
+        Types.KeyStoreException( message := "AWS KMS Key ARN does not match configured value")
+      );
 
-    var branchKeyRecord: versionBranchKeyItem := getItemResponse.Item.value;
+      var branchKey :- KMSKeystoreOperations.DecryptKey(
+        encryptionContext,
+        branchKeyItem[Structure.BRANCH_KEY_FIELD].B,
+        kmsConfiguration,
+        grantTokens,
+        kmsClient
+      );
 
-    var maybeBranchKeyResponse := decryptKeyStoreItem(branchKeyRecord, kmsKeyArn, grantTokens, logicalKeyStoreName, kmsClient);
-    var branchKeyResponse :- maybeBranchKeyResponse;
+      var branchKeyMaterials :- Structure.ToBranchKeyMaterials(
+        encryptionContext,
+        branchKey.Plaintext.value
+      );
 
-    var branchKeyVersion := branchKeyRecord["type"].S[|BRANCH_KEY_TYPE_PREFIX|..];
-    var branchKeyVersionUtf8 :- UTF8.Encode(branchKeyVersion).MapFailure(e => E(e));
-
-    return Success(Types.GetBranchKeyVersionOutput(
-                     branchKeyMaterials := Types.BranchKeyMaterials(
-                       branchKeyIdentifier := input.branchKeyIdentifier,
-                       branchKeyVersion := branchKeyVersionUtf8,
-                       branchKey := branchKeyResponse.Plaintext.value
-                     )
-                   ));
-  }
+      return Success(Types.GetBranchKeyVersionOutput(
+                       branchKeyMaterials := branchKeyMaterials
+                     ));
+    }
 
   method GetBeaconKeyAndUnwrap(
     input: Types.GetBeaconKeyInput,
     tableName: DDB.TableName,
     logicalKeyStoreName: string,
-    kmsKeyArn: Types.KmsKeyArn,
+    kmsConfiguration: Types.KMSConfiguration,
     grantTokens: KMS.GrantTokenList,
     kmsClient: KMS.IKMSClient,
     ddbClient: DDB.IDynamoDBClient
   )
-    returns (res: Result<Types.GetBeaconKeyOutput, Types.Error>)
+    returns (output: Result<Types.GetBeaconKeyOutput, Types.Error>)
     requires kmsClient.ValidState() && ddbClient.ValidState()
-    requires DDB.IsValid_TableName(tableName)
-    requires KMS.IsValid_KeyIdType(kmsKeyArn)
     modifies ddbClient.Modifies, kmsClient.Modifies
     ensures ddbClient.ValidState() && kmsClient.ValidState()
-  {
-    //= aws-encryption-sdk-specification/framework/key-store.md#getbeaconkey
-    //# MUST call AWS DDB `GetItem`
-    //# using the `branch-key-id` as the Partition Key and "beacon:true" value as the Sort Key.
-    var dynamoDbKey: DDB.Key := map[
-      BRANCH_KEY_IDENTIFIER_FIELD := DDB.AttributeValue.S(input.branchKeyIdentifier),
-      TYPE_FIELD := DDB.AttributeValue.S("beacon:true")
-    ];
-
-    var ItemRequest := DDB.GetItemInput(
-      Key := dynamoDbKey,
-      TableName := tableName,
-      AttributesToGet := None,
-      ConsistentRead :=  None,
-      ReturnConsumedCapacity := None,
-      ProjectionExpression := None,
-      ExpressionAttributeNames := None
-    );
-
-    var maybeGetItem := ddbClient.GetItem(ItemRequest);
-    var getItemResponse :- maybeGetItem
-    .MapFailure(e => Types.ComAmazonawsDynamodb(ComAmazonawsDynamodb := e));
-
-    :- Need(
-      getItemResponse.Item.Some?,
-      E("No item found for corresponding branch key identifier.")
-    );
-
-    :- Need(
-      //= aws-encryption-sdk-specification/framework/key-store.md#getbeaconkey
-      //# The AWS DDB response MUST contain the fields defined in the [branch keystore record format](../branch-key-store.md#record-format).
-      //# If the record does not contain the defined fields, this operation MUST fail.
-      //# If the record does not contain "SEARCH" as the "status" field, this operation MUST fail.
-      validBeaconKeyItem?(getItemResponse.Item.value),
-      E("Malformed Branch Key entry")
-    );
-
-    var beaconKeyItem: baseKeyStoreItem := getItemResponse.Item.value;
-    
-    //= aws-encryption-sdk-specification/framework/key-store.md#getbeaconkey
-    //# The operation MUST decrypt the beacon key according to the [AWS KMS Branch Key Decryption](#aws-kms-branch-key-decryption) section.
-    var beaconKeyResponse :- decryptKeyStoreItem(beaconKeyItem, kmsKeyArn, grantTokens, logicalKeyStoreName, kmsClient);
-
-    //= aws-encryption-sdk-specification/framework/key-store.md#getbeaconkey
-    //# This operation MUST return the constructed [beacon key materials](./structures.md#beacon-key-materials).
-    return Success(Types.GetBeaconKeyOutput(
-      //= aws-encryption-sdk-specification/framework/key-store.md#getbeaconkey
-      //# This operation MUST construct [beacon key materials](./structures.md#beacon-key-materials) from the decrypted branch key material
-      //# and the `branchKeyId` from the returned `branch-key-id` field.
-      beaconKeyMaterials := Types.BeaconKeyMaterials(
-        beaconKeyIdentifier := input.branchKeyIdentifier,
-        beaconKey := Some(beaconKeyResponse.Plaintext.value),
-        hmacKeys := None
-      )
-    ));
-  }
-
-  method decryptKeyStoreItem(
-    branchKeyRecord: baseKeyStoreItem,
-    awsKmsKeyArn: KMS.KeyIdType,
-    grantTokens: KMS.GrantTokenList,
-    logicalKeyStoreName: string,
-    kmsClient: KMS.IKMSClient
-  )
-    returns (output: Result<KMS.DecryptResponse, Types.Error>)
-    requires baseKeyStoreItemHasRequiredAttributes?(branchKeyRecord)
-    //= aws-encryption-sdk-specification/framework/key-store.md#aws-kms-branch-key-decryption
-    //= type=implication
-    //# The operation MUST use the configured `KMS SDK Client` to decrypt the value of the branch key field.
-    requires kmsClient.ValidState()
-    modifies kmsClient.Modifies
-    ensures kmsClient.ValidState()
-    ensures output.Success?
-      ==> 
-        && output.value.KeyId.Some?
-        //= aws-encryption-sdk-specification/framework/key-store.md#getbeaconkey
-        //= type=implication
-        //# - The `KeyId` field in the AWS KMS response MUST equal the configured AWS KMS Key ARN.
-        && output.value.KeyId.value == awsKmsKeyArn
-        && output.value.Plaintext.Some?
-        && 32 == |output.value.Plaintext.value|
-  {
-    var wrappedBranchKey: KMS.CiphertextType := branchKeyRecord[BRANCH_KEY_FIELD].B;
-
-    var encCtxDdbMap := branchKeyRecord - {BRANCH_KEY_FIELD};
-
-    var encCtxMap: map<string, string> :=
-      map k <- encCtxDdbMap ::
-        k := ValueToString(encCtxDdbMap[k]).value;
-    encCtxMap := encCtxMap + map[TABLE_FIELD := logicalKeyStoreName];
-
-    :- Need(
-      encCtxMap[KMS_FIELD] == awsKmsKeyArn,
-      Types.KeyStoreException(message := "Configured AWS KMS Key ARN does not match KMS Key ARN for branch-key-id: " + branchKeyRecord[BRANCH_KEY_IDENTIFIER_FIELD].S)
-    );
-
-    var decryptRequest :=
-      KMS.DecryptRequest(
-        //= aws-encryption-sdk-specification/framework/key-store.md#aws-kms-branch-key-decryption
-        //# `KeyId` MUST be the configured `AWS KMS Key ARN` in the [AWS KMS Configuration](#aws-kms-configuration) for this keystore
-        KeyId := Some(awsKmsKeyArn),
-        //= aws-encryption-sdk-specification/framework/key-store.md#aws-kms-branch-key-decryption
-        //# - `CiphertextBlob` MUST be the `enc` attribute value on the AWS DDB response item
-        CiphertextBlob := wrappedBranchKey,
-        //= aws-encryption-sdk-specification/framework/key-store.md#aws-kms-branch-key-decryption
-        //# - `EncryptionContext` MUST be the [encryption context](#encryption-context) constructed above
-        EncryptionContext := Some(encCtxMap),
-        //= aws-encryption-sdk-specification/framework/key-store.md#aws-kms-branch-key-decryption
-        //# - `GrantTokens` MUST be this keystore's [grant tokens](https://docs.aws.amazon.com/kms/latest/developerguide/concepts.html#grant_token).
-        GrantTokens := Some(grantTokens),
-        EncryptionAlgorithm := None
+    ensures output.Success? ==>
+              && input.branchKeyIdentifier == output.value.beaconKeyMaterials.beaconKeyIdentifier
+    {
+      var branchKeyItem :- DDBKeystoreOperations.GetBeaconKeyItem(
+        input.branchKeyIdentifier,
+        tableName,
+        ddbClient
       );
 
-    var maybeDecryptResponse := kmsClient.Decrypt(decryptRequest);
-    //= aws-encryption-sdk-specification/framework/key-store.md#getbeaconkey
-    //# If the beacon key fails to decrypt, this operation MUST fail.
-    var decryptResponse :- maybeDecryptResponse
-    .MapFailure(e => Types.ComAmazonawsKms(ComAmazonawsKms := e));
+      var encryptionContext := Structure.ToBranchKeyContext(branchKeyItem, logicalKeyStoreName);
 
-    :- Need(
-      && decryptResponse.KeyId.Some?
-      && decryptResponse.KeyId.value == awsKmsKeyArn
-      && decryptResponse.Plaintext.Some?
-      && 32 == |decryptResponse.Plaintext.value|,
-      E("Invalid response from KMS Decrypt")
-    );
-    return Success(decryptResponse);
-  }
+      :- Need(
+        KMSKeystoreOperations.AttemptKmsOperation?(kmsConfiguration, encryptionContext),
+        Types.KeyStoreException( message := "AWS KMS Key ARN does not match configured value")
+      );
 
-  method SortByTime(queryResponse: DDB.ItemList)
-    returns (output: branchKeyItem)
-    requires |queryResponse| > 0
-    requires
-      && (forall resp <- queryResponse ::
-            && validActiveBranchKey?(resp))
-    ensures validActiveBranchKey?(output)
-  {
-    if |queryResponse| == 1 {
-      return queryResponse[0];
+      var branchKey :- KMSKeystoreOperations.DecryptKey(
+        encryptionContext,
+        branchKeyItem[Structure.BRANCH_KEY_FIELD].B,
+        kmsConfiguration,
+        grantTokens,
+        kmsClient
+      );
+
+      var branchKeyMaterials :- Structure.ToBeaconKeyMaterials(
+        encryptionContext,
+        branchKey.Plaintext.value
+      );
+
+      return Success(Types.GetBeaconKeyOutput(
+                       beaconKeyMaterials := branchKeyMaterials
+                     ));
     }
 
-    var newestBranchKey: branchKeyItem := queryResponse[0];
-
-    for i := 1 to |queryResponse| {
-      var tmp: branchKeyItem := queryResponse[i];
-      var a := newestBranchKey["create-time"].S;
-      var b := tmp["create-time"].S;
-
-      if !LexicographicLessOrEqual(a, b, CharGreater) {
-        newestBranchKey := queryResponse[i];
-      } else {
-        if a == b {
-          var versionA := newestBranchKey["type"].S[|BRANCH_KEY_TYPE_PREFIX|..];
-          var versionB := tmp["type"].S[|BRANCH_KEY_TYPE_PREFIX|..];
-          if !LexicographicLessOrEqual(versionA, versionB, CharGreater) {
-            newestBranchKey := queryResponse[i];
-          }
-        }
-      }
-    }
-
-    return newestBranchKey;
-  }
-
-  function method CharGreater(a: char, b: char): bool
-  {
-    a > b
-  }
 }
