AwsCryptographicMaterialProviders/dafny/AwsCryptographyKeyStore/src/DDBKeystoreOperations.dfy
@@ -1,0 +1,141 @@
+include "../Model/AwsCryptographyKeyStoreTypes.dfy"
+include "Structure.dfy"
+
+module DDBKeystoreOperations {
+  import opened Wrappers
+  import opened UInt = StandardLibrary.UInt
+  import Seq
+  import Types = AwsCryptographyKeyStoreTypes
+  import DDB = ComAmazonawsDynamodbTypes
+  import UTF8
+  import Structure
+
+  method WriteNewKeyToStore(
+    versionBranchKeyItem: Structure.VersionBranchKeyItem,
+    activeBranchKeyItem: Structure.ActiveBranchKeyItem,
+    beaconKeyItem: Structure.BeaconKeyItem,
+    tableName: DDB.TableName,
+    ddbClient: DDB.IDynamoDBClient
+  )
+    returns (res: Result<DDB.TransactWriteItemsOutput, Types.Error>)
+    requires
+      && activeBranchKeyItem[Structure.BRANCH_KEY_IDENTIFIER_FIELD] == versionBranchKeyItem[Structure.BRANCH_KEY_IDENTIFIER_FIELD] == beaconKeyItem[Structure.BRANCH_KEY_IDENTIFIER_FIELD]
+      && activeBranchKeyItem[Structure.BRANCH_KEY_ACTIVE_VERSION_FIELD] == versionBranchKeyItem[Structure.TYPE_FIELD]
+    requires ddbClient.ValidState()
+    modifies ddbClient.Modifies
+    ensures ddbClient.ValidState()
+  // {
+  //   var branchKeyDDBMap := ToBranchKeyItemAttributeMap(branchKeyContext, wrappedBranchKey);
+  //   var branchKeyTransactWriteItem := CreateTransactWritePutItem(branchKeyDDBMap, tableName);
+
+  //   var beaconKeyDDBMap := ToBranchKeyItemAttributeMap(beaconKeyContext, wrappedBeaconKey);
+  //   var beaconKeyTransactWriteItem := CreateTransactWritePutItem(beaconKeyDDBMap, tableName);
+
+  //   :- Need(
+  //     // In order to be certain we are writing something that is well formed
+  //     // and something we will be able to get or query we need to ensure it has certain properties
+  //     && validBeaconKeyItem?(beaconKeyDDBMap)
+  //     && validActiveBranchKey?(branchKeyDDBMap),
+  //     Types.KeyStoreException(message := "Unable to write key material to Key Store: " + tableName)
+  //   );
+
+  //   var items: DDB.TransactWriteItemList := [
+  //     branchKeyTransactWriteItem,
+  //     beaconKeyTransactWriteItem
+  //   ];
+
+  //   var transactRequest := DDB.TransactWriteItemsInput(
+  //     TransactItems := items,
+  //     ReturnConsumedCapacity := None,
+  //     ReturnItemCollectionMetrics := None,
+  //     ClientRequestToken := None
+  //   );
+
+  //   var maybeTransactWriteResponse := ddbClient.TransactWriteItems(transactRequest);
+  //   var transactWriteItemsResponse :- maybeTransactWriteResponse
+  //   .MapFailure(e => Types.ComAmazonawsDynamodb(ComAmazonawsDynamodb := e));
+
+  //   res := Success(transactWriteItemsResponse);
+  // }
+
+
+  method WriteNewBranchKeyVersionToKeystore(
+    versionBranchKeyItem: Structure.VersionBranchKeyItem,
+    activeBranchKeyItem: Structure.ActiveBranchKeyItem,
+    tableName: DDB.TableName,
+    ddbClient: DDB.IDynamoDBClient
+  )
+    returns (res: Result<DDB.TransactWriteItemsOutput, Types.Error>)
+    requires
+      && activeBranchKeyItem[Structure.BRANCH_KEY_IDENTIFIER_FIELD] == versionBranchKeyItem[Structure.BRANCH_KEY_IDENTIFIER_FIELD]
+      && activeBranchKeyItem[Structure.BRANCH_KEY_ACTIVE_VERSION_FIELD] == versionBranchKeyItem[Structure.TYPE_FIELD]
+    requires ddbClient.ValidState()
+    modifies ddbClient.Modifies
+    ensures ddbClient.ValidState()
+  // {
+  // var decryptOnlyBranchKeyTransactWriteItem := CreateTransactWritePutItem(decryptOnlyBranchKey, tableName);
+  // var newActiveBranchKeyTransactWriteItem := CreateTransactWritePutItem(newActiveBranchKey, tableName);
+
+  // :- Need(
+  //   // In order to be certain we are writing something that is well formed
+  //   // and something we will be able to get or query we need to ensure it has certain properties
+  //   && validActiveBranchKey?(newActiveBranchKey)
+  //   && validVersionBranchKey?(decryptOnlyBranchKey),
+  //   Types.KeyStoreException(message := "Unable to write key material to Key Store: " + tableName)
+  // );
+
+  // var items: DDB.TransactWriteItemList := [
+  //   decryptOnlyBranchKeyTransactWriteItem,
+  //   newActiveBranchKeyTransactWriteItem
+  // ];
+
+  // var transactRequest := DDB.TransactWriteItemsInput(
+  //   TransactItems := items,
+  //   ReturnConsumedCapacity := None,
+  //   ReturnItemCollectionMetrics := None,
+  //   ClientRequestToken := None
+  // );
+
+  // var maybeTransactWriteResponse := ddbClient.TransactWriteItems(transactRequest);
+  // var transactWriteItemsResponse :- maybeTransactWriteResponse
+  // .MapFailure(e => Types.ComAmazonawsDynamodb(ComAmazonawsDynamodb := e));
+
+  // res := Success(transactWriteItemsResponse);
+  // }
+
+
+  method GetActiveBranchKeyItem(
+    branchKeyIdentifier: string,
+    tableName: DDB.TableName,
+    ddbClient: DDB.IDynamoDBClient
+  )
+    returns (res: Result<Structure.ActiveBranchKeyItem, Types.Error>)
+    requires DDB.IsValid_TableName(tableName)
+    requires ddbClient.ValidState()
+    modifies ddbClient.Modifies
+    ensures ddbClient.ValidState()
+
+  method GetVersionBranchKeyItem(
+    branchKeyIdentifier: string,
+    branchKeyVersion: string,
+    tableName: DDB.TableName,
+    ddbClient: DDB.IDynamoDBClient
+  )
+    returns (res: Result<Structure.VersionBranchKeyItem, Types.Error>)
+    requires DDB.IsValid_TableName(tableName)
+    requires ddbClient.ValidState()
+    modifies ddbClient.Modifies
+    ensures ddbClient.ValidState()
+
+  method GetBeaconKeyItem(
+    branchKeyIdentifier: string,
+    tableName: DDB.TableName,
+    ddbClient: DDB.IDynamoDBClient
+  )
+    returns (res: Result<Structure.BeaconKeyItem, Types.Error>)
+    requires DDB.IsValid_TableName(tableName)
+    requires ddbClient.ValidState()
+    modifies ddbClient.Modifies
+    ensures ddbClient.ValidState()
+
+}
