AwsCryptographicMaterialProviders/dafny/AwsCryptographyKeyStore/src/Structure.dfy
@@ -1,0 +1,273 @@
+// Copyright Amazon.com Inc. or its affiliates. All Rights Reserved.
+// SPDX-License-Identifier: Apache-2.0
+
+include "../Model/AwsCryptographyKeyStoreTypes.dfy"
+
+module Structure {
+  import opened Wrappers
+  import opened UInt = StandardLibrary.UInt
+  import Types = AwsCryptographyKeyStoreTypes
+  import DDB = ComAmazonawsDynamodbTypes
+  import KMS = ComAmazonawsKmsTypes
+  import UTF8
+
+  const KEY_CREATE_TIME := "create-time"
+  const HIERARCHY_VERSION := "hierarchy-version"
+  const TYPE_FIELD := "type"
+  const BRANCH_KEY_IDENTIFIER_FIELD := "branch-key-id"
+  const BRANCH_KEY_ACTIVE_VERSION_FIELD := "version"
+  const TABLE_FIELD := "tablename"
+  const KMS_FIELD := "kms-arn"
+  const BRANCH_KEY_FIELD := "enc"
+
+  const BRANCH_KEY_TYPE_PREFIX := "branch:version:"
+  const BRANCH_KEY_ACTIVE_TYPE := "branch:ACTIVE"
+  const BEACON_KEY_TYPE_VALUE := "beacon:ACTIVE"
+
+  // A GenerateDataKeyWithoutPlaintext of request size 32 returns a ciphertext size of 184 bytes.
+  const KMS_GEN_KEY_NO_PLAINTEXT_LENGTH_32 := 184
+
+  type BranchKeyContext = m: map<string, string> | BranchKeyContext?(m) witness *
+  predicate method BranchKeyContext?(m: map<string, string>) {
+    && BRANCH_KEY_IDENTIFIER_FIELD in m
+    && TYPE_FIELD in m
+    && KEY_CREATE_TIME in m
+    && HIERARCHY_VERSION in m
+    && TABLE_FIELD in m
+    && KMS_FIELD in m
+    && (forall k <- m.Keys :: DDB.IsValid_AttributeName(k))
+    && 0 < |m[BRANCH_KEY_IDENTIFIER_FIELD]|
+    && (BRANCH_KEY_ACTIVE_VERSION_FIELD in m ==>
+          && m[TYPE_FIELD] == BRANCH_KEY_ACTIVE_TYPE
+          && BRANCH_KEY_TYPE_PREFIX < m[BRANCH_KEY_ACTIVE_VERSION_FIELD])
+    && (BRANCH_KEY_ACTIVE_VERSION_FIELD !in m ==>
+          || m[TYPE_FIELD] == BEACON_KEY_TYPE_VALUE
+          || BRANCH_KEY_TYPE_PREFIX < m[TYPE_FIELD])
+    && BRANCH_KEY_FIELD !in m.Keys
+  }
+
+  // We specify that every item on the encryption context to KMS is stored in the branch/beacon key item.
+  // This method allows us to convert from a BranchKeyContext map to a DDB.AttributeMap easily.
+  function method ToAttributeMap(
+    encryptionContext: BranchKeyContext,
+    encryptedKey: seq<uint8>
+  ): (output: DDB.AttributeMap)
+    requires KMS.IsValid_CiphertextType(encryptedKey)
+    ensures BranchKeyItem?(output)
+  {
+    map k <- encryptionContext.Keys + {BRANCH_KEY_FIELD} - {TABLE_FIELD}
+      :: k := match k
+      case HIERARCHY_VERSION => DDB.AttributeValue.N(encryptionContext[HIERARCHY_VERSION])
+      case BRANCH_KEY_FIELD => DDB.AttributeValue.B(encryptedKey)
+      case _ => DDB.AttributeValue.S(encryptionContext[k])
+  }
+
+  function method ToBranchKeyContext(
+    item: DDB.AttributeMap,
+    logicalKeyStoreName: string
+  ): (output: BranchKeyContext)
+    requires BranchKeyItem?(item)
+  {
+    map k <- item.Keys + {TABLE_FIELD} - {BRANCH_KEY_FIELD}
+      :: k := match k
+      case HIERARCHY_VERSION => item[k].N
+      case TABLE_FIELD => logicalKeyStoreName
+      case _ => item[k].S
+  }
+
+  function method ToBranchKeyMaterials(
+    encryptionContext: BranchKeyContext,
+    plaintextKey: seq<uint8>
+  ): (output: Result<Types.BranchKeyMaterials, Types.Error>)
+    requires encryptionContext[TYPE_FIELD] != BEACON_KEY_TYPE_VALUE
+  {
+    var versionInformation := if BRANCH_KEY_ACTIVE_VERSION_FIELD in encryptionContext then
+                                encryptionContext[BRANCH_KEY_ACTIVE_VERSION_FIELD]
+                              else
+                                encryptionContext[TYPE_FIELD];
+    var branchKeyVersion := versionInformation[|BRANCH_KEY_TYPE_PREFIX|..];
+    var branchKeyVersionUtf8 :- UTF8.Encode(branchKeyVersion)
+    .MapFailure(e => Types.KeyStoreException( message := e ));
+
+    Success(Types.BranchKeyMaterials(
+              branchKeyIdentifier := encryptionContext[BRANCH_KEY_IDENTIFIER_FIELD],
+              branchKeyVersion := branchKeyVersionUtf8,
+              branchKey := plaintextKey
+            ))
+  }
+
+  function method ToBeaconKeyMaterials(
+    encryptionContext: BranchKeyContext,
+    plaintextKey: seq<uint8>
+  ): (output: Result<Types.BeaconKeyMaterials, Types.Error>)
+    requires encryptionContext[TYPE_FIELD] == BEACON_KEY_TYPE_VALUE
+  {
+
+    Success(Types.BeaconKeyMaterials(
+              beaconKeyIdentifier := encryptionContext[BRANCH_KEY_IDENTIFIER_FIELD],
+              beaconKey := Some(plaintextKey),
+              hmacKeys := None
+            ))
+  }
+
+  function method DecryptOnlyBranchKeyEncryptionContext(
+    branchKeyId: string,
+    branchKeyVersion: string,
+    timestamp: string,
+    logicalKeyStoreName: string,
+    kmsKeyArn: string
+  ): (output: map<string, string>)
+    requires 0 < |branchKeyId|
+    requires 0 < |branchKeyVersion|
+    ensures BranchKeyContext?(output)
+    ensures BRANCH_KEY_TYPE_PREFIX < output[TYPE_FIELD]
+    ensures BRANCH_KEY_ACTIVE_VERSION_FIELD !in output
+  {
+    map[
+      BRANCH_KEY_IDENTIFIER_FIELD := branchKeyId,
+      TYPE_FIELD := BRANCH_KEY_TYPE_PREFIX + branchKeyVersion,
+      KEY_CREATE_TIME := timestamp,
+      TABLE_FIELD := logicalKeyStoreName,
+      KMS_FIELD := kmsKeyArn,
+      HIERARCHY_VERSION := "1"
+    ]
+  }
+
+  function method ActiveBranchKeyEncryptionContext(
+    decryptOnlyEncryptionContext: map<string, string>
+  ): (output: map<string, string>)
+    requires BranchKeyContext?(decryptOnlyEncryptionContext)
+    requires
+      && BRANCH_KEY_TYPE_PREFIX < decryptOnlyEncryptionContext[TYPE_FIELD]
+      && BRANCH_KEY_ACTIVE_VERSION_FIELD !in decryptOnlyEncryptionContext
+    ensures BranchKeyContext?(output)
+    ensures BRANCH_KEY_ACTIVE_VERSION_FIELD in output
+  {
+    decryptOnlyEncryptionContext + map[
+      BRANCH_KEY_ACTIVE_VERSION_FIELD := decryptOnlyEncryptionContext[TYPE_FIELD],
+      TYPE_FIELD := BRANCH_KEY_ACTIVE_TYPE
+    ]
+  }
+
+  function method BeaconKeyEncryptionContext(
+    decryptOnlyEncryptionContext: map<string, string>
+  ): (output: map<string, string>)
+    requires BranchKeyContext?(decryptOnlyEncryptionContext)
+    requires
+      && BRANCH_KEY_TYPE_PREFIX < decryptOnlyEncryptionContext[TYPE_FIELD]
+      && BRANCH_KEY_ACTIVE_VERSION_FIELD !in decryptOnlyEncryptionContext
+    ensures BranchKeyContext?(output)
+    ensures output[TYPE_FIELD] == BEACON_KEY_TYPE_VALUE
+  {
+    decryptOnlyEncryptionContext + map[
+      TYPE_FIELD := BEACON_KEY_TYPE_VALUE
+    ]
+  }
+
+  // function method GetBranchKeyVersion(
+  //   encryptionContext: BranchKeyContext,
+  // ): (version: Result<string, Types.Error>)
+  //   requires BranchKeyContext?(decryptOnlyEncryptionContext)
+
+  predicate method BranchKeyItem?(m: DDB.AttributeMap) {
+    && BRANCH_KEY_IDENTIFIER_FIELD in m && m[BRANCH_KEY_IDENTIFIER_FIELD].S?
+    && 0 < |m[BRANCH_KEY_IDENTIFIER_FIELD].S|
+    && TYPE_FIELD in m && m[TYPE_FIELD].S?
+    && KEY_CREATE_TIME in m && m[KEY_CREATE_TIME].S?
+    && HIERARCHY_VERSION in m && m[HIERARCHY_VERSION].N?
+    && KMS_FIELD in m && m[KMS_FIELD].S?
+    && (BRANCH_KEY_ACTIVE_VERSION_FIELD in m ==>
+          && m[TYPE_FIELD].S? && m[BRANCH_KEY_ACTIVE_VERSION_FIELD].S?
+          && m[TYPE_FIELD].S == BRANCH_KEY_ACTIVE_TYPE
+          && BRANCH_KEY_TYPE_PREFIX < m[BRANCH_KEY_ACTIVE_VERSION_FIELD].S
+       )
+    && (BRANCH_KEY_ACTIVE_VERSION_FIELD !in m ==>
+          && m[TYPE_FIELD].S?
+          && (m[TYPE_FIELD].S == BEACON_KEY_TYPE_VALUE || BRANCH_KEY_TYPE_PREFIX < m[TYPE_FIELD].S)
+       )
+    && BRANCH_KEY_FIELD in m && m[BRANCH_KEY_FIELD].B?
+    && KMS.IsValid_CiphertextType(m[BRANCH_KEY_FIELD].B)
+    && (forall k <- m.Keys - {BRANCH_KEY_FIELD, HIERARCHY_VERSION} :: m[k].S?)
+  }
+
+  type ActiveBranchKeyItem = m: DDB.AttributeMap | ActiveBranchKeyItem?(m) witness *
+  predicate method ActiveBranchKeyItem?(m: DDB.AttributeMap) {
+    && BranchKeyItem?(m)
+    && m[TYPE_FIELD].S == BRANCH_KEY_ACTIVE_TYPE
+    && BRANCH_KEY_ACTIVE_VERSION_FIELD in m && m[BRANCH_KEY_ACTIVE_VERSION_FIELD].S?
+    && BRANCH_KEY_TYPE_PREFIX < m[BRANCH_KEY_ACTIVE_VERSION_FIELD].S
+  }
+
+  type VersionBranchKeyItem = m: DDB.AttributeMap | VersionBranchKeyItem?(m) witness *
+  predicate method VersionBranchKeyItem?(m: DDB.AttributeMap) {
+    && BranchKeyItem?(m)
+    && BRANCH_KEY_ACTIVE_VERSION_FIELD !in m
+    && BRANCH_KEY_TYPE_PREFIX < m[TYPE_FIELD].S
+  }
+
+  type BeaconKeyItem = m: DDB.AttributeMap | BeaconKeyItem?(m) witness *
+  predicate method BeaconKeyItem?(m: DDB.AttributeMap) {
+    && BranchKeyItem?(m)
+    && BRANCH_KEY_ACTIVE_VERSION_FIELD !in m
+    && m[TYPE_FIELD].S == BEACON_KEY_TYPE_VALUE
+  }
+
+  lemma BranchKeyItemsDoNotCollide(a: ActiveBranchKeyItem, b: VersionBranchKeyItem, c: BeaconKeyItem)
+    requires a[BRANCH_KEY_IDENTIFIER_FIELD] == b[BRANCH_KEY_IDENTIFIER_FIELD] == c[BRANCH_KEY_IDENTIFIER_FIELD]
+    ensures a[TYPE_FIELD] != b[TYPE_FIELD]
+    ensures a[TYPE_FIELD] != c[TYPE_FIELD]
+    ensures c[TYPE_FIELD] != b[TYPE_FIELD]
+  {}
+
+  lemma ToAttributeMapIsCorrect(
+    encryptionContext: BranchKeyContext,
+    encryptedKey: seq<uint8>,
+    item: DDB.AttributeMap
+  )
+    requires KMS.IsValid_CiphertextType(encryptedKey)
+    requires item == ToAttributeMap(encryptionContext, encryptedKey)
+    ensures item.Keys == encryptionContext.Keys + {BRANCH_KEY_FIELD} - {TABLE_FIELD}
+    ensures item[BRANCH_KEY_FIELD].B == encryptedKey
+    ensures
+      && (forall k <- item.Keys - {BRANCH_KEY_FIELD, HIERARCHY_VERSION}
+      ::
+        && item[k].S?
+        && encryptionContext[k] == item[k].S
+      )
+      && encryptionContext[HIERARCHY_VERSION] == item[HIERARCHY_VERSION].N
+  {}
+
+  lemma EncryptionContextConstructorsAreCorrect(
+    branchKeyId: string,
+    branchKeyVersion: string,
+    timestamp: string,
+    logicalKeyStoreName: string,
+    kmsKeyArn: string
+    )
+    requires 0 < |branchKeyId|
+    requires 0 < |branchKeyVersion|
+
+    ensures
+      var decryptOnly := DecryptOnlyBranchKeyEncryptionContext(branchKeyId, branchKeyVersion, timestamp, logicalKeyStoreName, kmsKeyArn);
+      var active := ActiveBranchKeyEncryptionContext(decryptOnly);
+      var beacon := BeaconKeyEncryptionContext(decryptOnly);
+      && decryptOnly[TYPE_FIELD] != active[TYPE_FIELD]
+      && decryptOnly[TYPE_FIELD] != beacon[TYPE_FIELD]
+      && active[TYPE_FIELD] != beacon[TYPE_FIELD]
+      && (forall k <- decryptOnly.Keys - {TYPE_FIELD} ::
+        && decryptOnly[k] == active[k] == beacon[k]
+        )
+      && active[BRANCH_KEY_ACTIVE_VERSION_FIELD] == decryptOnly[TYPE_FIELD]
+  {}
+
+  lemma ToAttributeMapAndToBranchKeyContextAreInverse(
+    encryptionContext: BranchKeyContext,
+    encryptedKey: seq<uint8>,
+    item: DDB.AttributeMap
+  )
+    requires KMS.IsValid_CiphertextType(encryptedKey)
+    requires item == ToAttributeMap(encryptionContext, encryptedKey)
+    ensures ToBranchKeyContext(item, encryptionContext[TABLE_FIELD]) == encryptionContext
+  {}
+
+}
